config.el
@@ -1,0 +1,1 @@
+(add-to-list 'coq-load-path (list (expand-file-name "coq") "LCAC"))
