coq/config.el
@@ -1,1 +1,0 @@
-(add-to-list 'coq-load-path (list (expand-file-name default-directory) "LCAC"))
